coq/theories/parsing/Parser.v
@@ -6,6 +6,7 @@ Require Import impboot.parsing.ParserData.
 Require Import impboot.imp2asm.ImpToASMCodegen.
 Require Import impboot.imperative.ImpSyntax.
 Require Import impboot.functional.FunValues.
+Require Import impboot.commons.PrintingUtils.
 Require Import coqutil.Word.Interface.
 Require Import coqutil.Word.Properties.
 
@@ -160,27 +161,26 @@ Definition lexer (input: string): list token :=
 
 (* parsing *)
 
-Definition quote n :=
-  let/d quote_str := "'" in
-  let/d quote_enc := name_enc quote_str in
+Definition quote (n: N) :=
+  let/d quote_enc := name_enc "'" in
   let/d quote_num := Num quote_enc in
   let/d n_num := Num n in
   let/d pair_list := [quote_num; n_num] in
   let/d result := FunValues.vlist pair_list in
   result.
 
-Fixpoint parse (ts: list token) (x: Value) (s: list Value) :=
+Fixpoint parse (ts: list token) (x: Value) (stck: list Value) :=
   match ts with
   | [] => x
   | (CLOSE :: rest) => 
     let/d zero_num := Num 0 in
-    let/d x_cons_s := x :: s in
+    let/d x_cons_s := x :: stck in
     let/d result := parse rest zero_num x_cons_s in
     result
   | (OPEN :: rest) =>
-    match s with
+    match stck with
     | [] => 
-      let/d result := parse rest x s in
+      let/d result := parse rest x stck in
       result
     | (y :: ys) => 
       let/d pair_x_y := Pair x y in
@@ -190,16 +190,16 @@ Fixpoint parse (ts: list token) (x: Value) (s: list Value) :=
   | (NUM n :: rest) => 
     let/d n_num := Num n in
     let/d pair_n_x := Pair n_num x in
-    let/d result := parse rest pair_n_x s in
+    let/d result := parse rest pair_n_x stck in
     result
   | (QUOTE n :: rest) => 
     let/d quote_n := quote n in
     let/d pair_quote_x := Pair quote_n x in
-    let/d result := parse rest pair_quote_x s in
+    let/d result := parse rest pair_quote_x stck in
     result
   | (DOT :: rest) => 
     let/d vhead_x := FunValues.vhead x in
-    let/d result := parse rest vhead_x s in
+    let/d result := parse rest vhead_x stck in
     result
   end.
 Theorem parse_equation: ltac2:(unfold_fix_type '@parse).
@@ -207,7 +207,7 @@ Proof. unfold_fix_proof '@parse. Qed.
 
 (* converting from v to prog *)
 
-Fixpoint v2list v :=
+Fixpoint v2list (v: FunValues.Value) :=
   match v with
   | Num _ => 
     let/d empty_list := [] in
@@ -220,11 +220,11 @@ Fixpoint v2list v :=
 Theorem v2list_equation: ltac2:(unfold_fix_type '@v2list).
 Proof. unfold_fix_proof '@v2list. Qed.
 
-Definition num2exp n :=
+Definition num2exp (n: N) :=
   let/d is_upper := vis_upper n in
   if is_upper then 
-    let/d n_z := Z.of_N n in
-    let/d word_val := word.of_Z n_z in
+    let/d n1 := N_modulo n (2 ^ 64) in
+    let/d word_val := word.of_Z (Z.of_N n1) in
     let/d result := ImpSyntax.Const word_val in
     result
   else 
@@ -243,70 +243,48 @@ Fixpoint v2exp (v: Value): ImpSyntax.exp :=
       let/d result := num2exp n in (* fail? *)
       result
     | Pair v1 v2 =>
-      let/d quote_str := "'" in
-      let/d quote_enc := name_enc quote_str in
-      let/d is_quote := N.eqb n quote_enc in
-      if is_quote then 
+      if N.eqb n (name_enc "'") then 
         let/d v1_num := vgetNum v1 in
-        let/d v1_z := Z.of_N v1_num in
-        let/d word_val := word.of_Z v1_z in
+        let/d v1_num_mod := N_modulo v1_num (2 ^ 64) in
+        let/d word_val := word.of_Z (Z.of_N v1_num_mod) in
         let/d result := Const word_val in
         result
+      else if N.eqb n (name_enc "var") then 
+        let/d v1_num := vgetNum v1 in
+        let/d result := Var v1_num in
+        result
       else
-        let/d var_str := "var" in
-        let/d var_enc := name_enc var_str in
-        let/d is_var := N.eqb n var_enc in
-        if is_var then 
-          let/d v1_num := vgetNum v1 in
-          let/d result := Var v1_num in
+        match v2 with
+        | Num _ => 
+          let/d result := num2exp n in (* fail? *)
           result
-        else
-          match v2 with
-          | Num _ => 
-            let/d result := num2exp n in (* fail? *)
+        | Pair v2 v3 =>
+          if N.eqb n (name_enc "+") then 
+            let/d v1_exp := v2exp v1 in
+            let/d v2_exp := v2exp v2 in
+            let/d result := Add v1_exp v2_exp in
             result
-          | Pair v2 v3 =>
-            let/d plus_str := "+" in
-            let/d plus_enc := name_enc plus_str in
-            let/d is_plus := N.eqb n plus_enc in
-            if is_plus then 
-              let/d v1_exp := v2exp v1 in
-              let/d v2_exp := v2exp v2 in
-              let/d result := Add v1_exp v2_exp in
-              result
-            else
-              let/d minus_str := "-" in
-              let/d minus_enc := name_enc minus_str in
-              let/d is_minus := N.eqb n minus_enc in
-              if is_minus then 
-                let/d v1_exp := v2exp v1 in
-                let/d v2_exp := v2exp v2 in
-                let/d result := Sub v1_exp v2_exp in
-                result
-              else
-                let/d div_str := "div" in
-                let/d div_enc := name_enc div_str in
-                let/d is_div := N.eqb n div_enc in
-                if is_div then 
-                  let/d v1_exp := v2exp v1 in
-                  let/d v2_exp := v2exp v2 in
-                  let/d result := Div v1_exp v2_exp in
-                  result
-                else
-                  let/d read_str := "read" in
-                  let/d read_enc := name_enc read_str in
-                  let/d is_read := N.eqb n read_enc in
-                  if is_read then 
-                    let/d v1_exp := v2exp v1 in
-                    let/d v2_exp := v2exp v2 in
-                    let/d result := Read v1_exp v2_exp in
-                    result
-                  else
-                    let/d vel0_v := vel0 v in
-                    let/d vel0_num := vgetNum vel0_v in
-                    let/d result := Var vel0_num in (* fail? *)
-                    result
-          end
+          else if N.eqb n (name_enc "-") then 
+            let/d v1_exp := v2exp v1 in
+            let/d v2_exp := v2exp v2 in
+            let/d result := Sub v1_exp v2_exp in
+            result
+          else if N.eqb n (name_enc "div") then 
+            let/d v1_exp := v2exp v1 in
+            let/d v2_exp := v2exp v2 in
+            let/d result := Div v1_exp v2_exp in
+            result
+          else if N.eqb n (name_enc "read") then 
+            let/d v1_exp := v2exp v1 in
+            let/d v2_exp := v2exp v2 in
+            let/d result := Read v1_exp v2_exp in
+            result
+          else
+            let/d vel0_v := vel0 v in
+            let/d vel0_num := vgetNum vel0_v in
+            let/d result := Var vel0_num in (* fail? *)
+            result
+        end
     end
   end.
 Theorem v2exp_equation: ltac2:(unfold_fix_type '@v2exp).
@@ -328,24 +306,17 @@ Proof. unfold_fix_proof '@vs2exps. Qed.
 
 Definition v2cmp (v: Value): ImpSyntax.cmp :=
   let/d v_num := vgetNum v in
-  let/d less_str := "<" in
-  let/d less_enc := name_enc less_str in
-  let/d is_less := N.eqb v_num less_enc in
-  if is_less then 
+  if N.eqb v_num (name_enc "<") then 
     Less 
+  else if N.eqb v_num (name_enc "=") then 
+    Equal
   else
-    let/d equal_str := "=" in
-    let/d equal_enc := name_enc equal_str in
-    let/d is_equal := N.eqb v_num equal_enc in
-    if is_equal then 
-      Equal 
-    else
-      Less. (* fail? *)
+    Less. (* fail? *)
 
 Fixpoint v2test (v: Value): ImpSyntax.test :=
   match v with
   | Num _ => 
-    let/d zero_word := word.of_Z 0 in
+    let/d zero_word := word.of_Z (Z.of_N 0) in
     let/d zero_const := Const zero_word in
     let/d result := Test Less zero_const zero_const in (* fail? *)
     result
@@ -353,49 +324,39 @@ Fixpoint v2test (v: Value): ImpSyntax.test :=
     let/d n := vgetNum v0 in (* this can fail? *)
     match v1 return ImpSyntax.test with
     | Num _ => 
-      let/d zero_word := word.of_Z 0 in
+      let/d zero_word := word.of_Z (Z.of_N 0) in
       let/d zero_const := Const zero_word in
       let/d result := Test Less zero_const zero_const in (* fail? *)
       result
     | Pair v1 v2 =>
-      let/d not_str := "not" in
-      let/d not_enc := name_enc not_str in
-      let/d is_not := N.eqb n not_enc in
-      if is_not then 
+      if N.eqb n (name_enc "not") then 
         let/d v1_test := v2test v1 in
         let/d result := Not v1_test in
         result
       else
         match v2 with
         | Num _ => 
-          let/d zero_word := word.of_Z 0 in
+          let/d zero_word := word.of_Z (Z.of_N 0) in
           let/d zero_const := Const zero_word in
           let/d result := Test Less zero_const zero_const in (* fail? *)
           result
         | Pair v2 v3 =>
-          let/d and_str := "and" in
-          let/d and_enc := name_enc and_str in
-          let/d is_and := N.eqb n and_enc in
-          if is_and then 
+          if N.eqb n (name_enc "and") then 
             let/d v1_test := v2test v1 in
             let/d v2_test := v2test v2 in
             let/d result := And v1_test v2_test in
             result
+          else if N.eqb n (name_enc "or") then 
+            let/d v1_test := v2test v1 in
+            let/d v2_test := v2test v2 in
+            let/d result := Or v1_test v2_test in
+            result
           else
-            let/d or_str := "or" in
-            let/d or_enc := name_enc or_str in
-            let/d is_or := N.eqb n or_enc in
-            if is_or then 
-              let/d v1_test := v2test v1 in
-              let/d v2_test := v2test v2 in
-              let/d result := Or v1_test v2_test in
-              result
-            else
-              let/d v0_cmp := v2cmp v0 in
-              let/d v1_exp := v2exp v1 in
-              let/d v2_exp := v2exp v2 in
-              let/d result := Test v0_cmp v1_exp v2_exp in
-              result
+            let/d v0_cmp := v2cmp v0 in
+            let/d v1_exp := v2exp v1 in
+            let/d v2_exp := v2exp v2 in
+            let/d result := Test v0_cmp v1_exp v2_exp in
+            result
         end
     end
   end.
@@ -406,134 +367,96 @@ Fixpoint v2cmd (v: Value): ImpSyntax.cmd :=
   match v with
   | Num _ => Skip
   | Pair v0 v1 =>
-    match v0 with
-    | Pair _ _ =>
-      match v1 with
-      | Num _ => 
+    let/d iPv0 := visPair v0 in
+    if iPv0 then
+      let/d iNv1 := visNum v1 in
+      if iNv1 then
         let/d result := v2cmd v0 in
         result
-      | Pair _ _ =>
+      else
         let/d v0_cmd := v2cmd v0 in
         let/d v1_cmd := v2cmd v1 in
         let/d result := Seq v0_cmd v1_cmd in
         result
-      end
-    | Num _ =>
+    else
       let/d n := vgetNum v0 in
-      let/d abort_str := "abort" in
-      let/d abort_enc := name_enc abort_str in
-      let/d is_abort := N.eqb n abort_enc in
-      if is_abort then 
-        Abort 
+      if N.eqb n (name_enc "abort") then
+        Abort
       else
         match v1 with
         | Num _ => Skip (* fail? *)
         | Pair v1 v2 =>
-          let/d return_str := "return" in
-          let/d return_enc := name_enc return_str in
-          let/d is_return := N.eqb n return_enc in
-          if is_return then 
+          if N.eqb n (name_enc "return") then
             let/d v1_exp := v2exp v1 in
             let/d result := Return v1_exp in
             result
+          else if N.eqb n (name_enc "getchar") then
+            let/d v1_num := vgetNum v1 in
+            let/d result := GetChar v1_num in
+            result
+          else if N.eqb n (name_enc "putchar") then
+            let/d v1_exp := v2exp v1 in
+            let/d result := PutChar v1_exp in
+            result
           else
-            let/d getchar_str := "getchar" in
-            let/d getchar_enc := name_enc getchar_str in
-            let/d is_getchar := N.eqb n getchar_enc in
-            if is_getchar then 
-              let/d v1_num := vgetNum v1 in
-              let/d result := GetChar v1_num in
-              result
-            else
-              let/d putchar_str := "putchar" in
-              let/d putchar_enc := name_enc putchar_str in
-              let/d is_putchar := N.eqb n putchar_enc in
-              if is_putchar then 
-                let/d v1_exp := v2exp v1 in
-                let/d result := PutChar v1_exp in
+            match v2 with
+            | Num n2 => Skip (* fail? *)
+            | Pair v2 v3 =>
+              if N.eqb n (name_enc "assign") then
+                let/d v1_num := vgetNum v1 in
+                let/d v2_exp := v2exp v2 in
+                let/d result := Assign v1_num v2_exp in
+                result
+              else if N.eqb n (name_enc "while") then
+                let/d v1_test := v2test v1 in
+                let/d v2_cmd := v2cmd v2 in
+                let/d result := While v1_test v2_cmd in
+                result
+              else if N.eqb n (name_enc "alloc") then
+                let/d v1_num := vgetNum v1 in
+                let/d v2_exp := v2exp v2 in
+                let/d result := Alloc v1_num v2_exp in
                 result
               else
-                match v2 with
-                | Num n2 => Skip (* fail? *)
-                | Pair v2 v3 =>
-                  let/d assign_str := "assign" in
-                  let/d assign_enc := name_enc assign_str in
-                  let/d is_assign := N.eqb n assign_enc in
-                  if is_assign then 
-                    let/d v1_num := vgetNum v1 in
+                match v3 with
+                | Num _ =>
+                  let/d v0_num := vgetNum v0 in
+                  let/d v1_num := vgetNum v1 in
+                  let/d v2_list := v2list v2 in
+                  let/d v2_exps := vs2exps v2_list in
+                  let/d result := Call v0_num v1_num v2_exps in
+                  result
+                | Pair v3 v4 =>
+                  if N.eqb n (name_enc "update") then
+                    let/d v1_exp := v2exp v1 in
                     let/d v2_exp := v2exp v2 in
-                    let/d result := Assign v1_num v2_exp in
+                    let/d v3_exp := v2exp v3 in
+                    let/d result := Update v1_exp v2_exp v3_exp in
+                    result
+                  else if N.eqb n (name_enc "if") then
+                    let/d v1_test := v2test v1 in
+                    let/d v2_cmd := v2cmd v2 in
+                    let/d v3_cmd := v2cmd v3 in
+                    let/d result := If v1_test v2_cmd v3_cmd in
+                    result
+                  else if N.eqb n (name_enc "call") then
+                    let/d v1_num := vgetNum v1 in
+                    let/d v2_num := vgetNum v2 in
+                    let/d v3_list := v2list v3 in
+                    let/d v3_exps := vs2exps v3_list in
+                    let/d result := Call v1_num v2_num v3_exps in
                     result
                   else
-                    let/d while_str := "while" in
-                    let/d while_enc := name_enc while_str in
-                    let/d is_while := N.eqb n while_enc in
-                    if is_while then 
-                      let/d v1_test := v2test v1 in
-                      let/d v2_cmd := v2cmd v2 in
-                      let/d result := While v1_test v2_cmd in
-                      result
-                    else
-                      let/d alloc_str := "alloc" in
-                      let/d alloc_enc := name_enc alloc_str in
-                      let/d is_alloc := N.eqb n alloc_enc in
-                      if is_alloc then 
-                        let/d v1_num := vgetNum v1 in
-                        let/d v2_exp := v2exp v2 in
-                        let/d result := Alloc v1_num v2_exp in
-                        result
-                      else
-                        match v3 with
-                        | Num _ =>
-                          let/d v0_num := vgetNum v0 in
-                          let/d v1_num := vgetNum v1 in
-                          let/d v2_list := v2list v2 in
-                          let/d v2_exps := vs2exps v2_list in
-                          let/d result := Call v0_num v1_num v2_exps in
-                          result
-                        | Pair v3 v4 =>
-                          let/d update_str := "update" in
-                          let/d update_enc := name_enc update_str in
-                          let/d is_update := N.eqb n update_enc in
-                          if is_update then 
-                            let/d v1_exp := v2exp v1 in
-                            let/d v2_exp := v2exp v2 in
-                            let/d v3_exp := v2exp v3 in
-                            let/d result := Update v1_exp v2_exp v3_exp in
-                            result
-                          else
-                            let/d if_str := "if" in
-                            let/d if_enc := name_enc if_str in
-                            let/d is_if := N.eqb n if_enc in
-                            if is_if then 
-                              let/d v1_test := v2test v1 in
-                              let/d v2_cmd := v2cmd v2 in
-                              let/d v3_cmd := v2cmd v3 in
-                              let/d result := If v1_test v2_cmd v3_cmd in
-                              result
-                            else
-                              let/d call_str := "call" in
-                              let/d call_enc := name_enc call_str in
-                              let/d is_call := N.eqb n call_enc in
-                              if is_call then 
-                                let/d v1_num := vgetNum v1 in
-                                let/d v2_num := vgetNum v2 in
-                                let/d v3_list := v2list v3 in
-                                let/d v3_exps := vs2exps v3_list in
-                                let/d result := Call v1_num v2_num v3_exps in
-                                result
-                              else
-                                let/d v0_num := vgetNum v0 in
-                                let/d v1_num := vgetNum v1 in
-                                let/d v2_v3_pair := Pair v2 v3 in
-                                let/d pair_list := v2list v2_v3_pair in
-                                let/d pair_exps := vs2exps pair_list in
-                                let/d result := Call v0_num v1_num pair_exps in
-                                result
-                        end
+                    let/d v0_num := vgetNum v0 in
+                    let/d v1_num := vgetNum v1 in
+                    let/d v2_v3_pair := Pair v2 v3 in
+                    let/d pair_list := v2list v2_v3_pair in
+                    let/d pair_exps := vs2exps pair_list in
+                    let/d result := Call v0_num v1_num pair_exps in
+                    result
                 end
+            end
         end
-    end
   end.
 Theorem v2cmd_equation: ltac2:(unfold_fix_type '@v2cmd).
 Proof. unfold_fix_proof '@v2cmd. Qed.
@@ -592,8 +515,8 @@ Definition parser (tokens: list token): prog :=
   let/d result := vs2prog val_list in
   result.
 
-Definition str2imp (s: string): ImpSyntax.prog :=
-  let/d toks := lexer s in
+Definition str2imp (str: string): ImpSyntax.prog :=
+  let/d toks := lexer str in
   let/d prog := parser toks in
   let/d result := prog in
   result.
