coq/theories/derivations/ParserDerivations.v
@@ -22,7 +22,7 @@ From Ltac2 Require Import Ltac2.
 
 (* lexing *)
 
-Derive read_num_prog
+(* Derive read_num_prog
   in ltac2:(relcompile_tpe 'read_num_prog 'read_num [])
   as read_num_prog_proof.
 Proof.
@@ -62,19 +62,87 @@ Derive lexer_prog
   as lexer_prog_proof.
 Proof.
   time relcompile.
+Qed. *)
+
+(* FunValues *)
+
+Derive vcons_prog
+  in ltac2:(relcompile_tpe 'vcons_prog 'vcons [])
+  as vcons_prog_proof.
+Proof.
+  time relcompile.
+Qed.
+
+Derive vhead_prog
+  in ltac2:(relcompile_tpe 'vhead_prog 'vhead [])
+  as vhead_prog_proof.
+Proof.
+  time relcompile.
+Qed.
+
+Derive vlist_prog
+  in ltac2:(relcompile_tpe 'vlist_prog 'vlist ['vcons])
+  as vlist_prog_proof.
+Proof.
+  time relcompile.
+Qed.
+
+Theorem vis_upper_f_equation: ltac2:(unfold_fix_type '@vis_upper_f).
+Proof. unfold_fix_proof '@vis_upper_f. Qed.
+Derive vis_upper_f_prog
+  in ltac2:(relcompile_tpe 'vis_upper_f_prog 'vis_upper_f [])
+  as vis_upper_f_prog_proof.
+Proof.
+  time relcompile.
+  ltac1:(lia).
+Qed.
+
+Derive vis_upper_prog
+  in ltac2:(relcompile_tpe 'vis_upper_prog 'vis_upper ['vis_upper_f])
+  as vis_upper_prog_proof.
+Proof.
+  time relcompile.
+Qed.
+
+Derive vgetNum_prog
+  in ltac2:(relcompile_tpe 'vgetNum_prog 'vgetNum [])
+  as vgetNum_prog_proof.
+Proof.
+  time relcompile.
+Qed.
+
+Derive vel0_prog
+  in ltac2:(relcompile_tpe 'vel0_prog 'vel0 ['vhead])
+  as vel0_prog_proof.
+Proof.
+  time relcompile.
+Qed.
+
+Derive visNum_prog
+  in ltac2:(relcompile_tpe 'visNum_prog 'visNum [])
+  as visNum_prog_proof.
+Proof.
+  time relcompile.
+Qed.
+
+Derive visPair_prog
+  in ltac2:(relcompile_tpe 'visPair_prog 'visPair [])
+  as visPair_prog_proof.
+Proof.
+  time relcompile.
 Qed.
 
 (* parsing *)
 
 Derive quote_prog
-  in ltac2:(relcompile_tpe 'quote_prog 'quote [])
+  in ltac2:(relcompile_tpe 'quote_prog 'quote ['vlist])
   as quote_prog_proof.
 Proof.
   time relcompile.
 Qed.
 
 Derive parse_prog
-  in ltac2:(relcompile_tpe 'parse_prog 'parse [])
+  in ltac2:(relcompile_tpe 'parse_prog 'parse ['vhead; 'quote])
   as parse_prog_proof.
 Proof.
   time relcompile.
@@ -90,70 +158,72 @@ Proof.
 Qed.
 
 Derive num2exp_prog
-  in ltac2:(relcompile_tpe 'num2exp_prog 'num2exp [])
+  in ltac2:(relcompile_tpe 'num2exp_prog 'num2exp ['vis_upper; 'N_modulo])
   as num2exp_prog_proof.
 Proof.
   time relcompile.
+  subst; eapply N_modulo_lt; ltac1:(lia).
 Qed.
 
 Derive v2exp_prog
-  in ltac2:(relcompile_tpe 'v2exp_prog 'v2exp [])
+  in ltac2:(relcompile_tpe 'v2exp_prog 'v2exp ['vgetNum; 'vel0; 'num2exp; 'N_modulo])
   as v2exp_prog_proof.
 Proof.
   time relcompile.
+  subst; eapply N_modulo_lt; ltac1:(lia).
 Qed.
 
 Derive vs2exps_prog
-  in ltac2:(relcompile_tpe 'vs2exps_prog 'vs2exps [])
+  in ltac2:(relcompile_tpe 'vs2exps_prog 'vs2exps ['v2exp])
   as vs2exps_prog_proof.
 Proof.
   time relcompile.
 Qed.
 
 Derive v2cmp_prog
-  in ltac2:(relcompile_tpe 'v2cmp_prog 'v2cmp [])
+  in ltac2:(relcompile_tpe 'v2cmp_prog 'v2cmp ['vgetNum])
   as v2cmp_prog_proof.
 Proof.
   time relcompile.
 Qed.
 
 Derive v2test_prog
-  in ltac2:(relcompile_tpe 'v2test_prog 'v2test [])
+  in ltac2:(relcompile_tpe 'v2test_prog 'v2test ['vgetNum; 'v2cmp; 'v2exp])
   as v2test_prog_proof.
 Proof.
   time relcompile.
 Qed.
 
 Derive v2cmd_prog
-  in ltac2:(relcompile_tpe 'v2cmd_prog 'v2cmd [])
+  in ltac2:(relcompile_tpe 'v2cmd_prog 'v2cmd ['vgetNum; 'v2exp; 'v2test; 'v2list; 'vs2exps; 'visNum; 'visPair])
   as v2cmd_prog_proof.
 Proof.
   time relcompile.
 Qed.
 
 Derive vs2args_prog
-  in ltac2:(relcompile_tpe 'vs2args_prog 'vs2args [])
+  in ltac2:(relcompile_tpe 'vs2args_prog 'vs2args ['vgetNum])
   as vs2args_prog_proof.
 Proof.
   time relcompile.
 Qed.
 
 Derive v2func_prog
-  in ltac2:(relcompile_tpe 'v2func_prog 'v2func [])
+  in ltac2:(relcompile_tpe 'v2func_prog 'v2func ['vel1; 'vel2; 'vel3; 'vgetNum; 'v2list; 'vs2args; 'v2cmd])
   as v2func_prog_proof.
 Proof.
   time relcompile.
 Qed.
 
 Derive v2funcs_prog
-  in ltac2:(relcompile_tpe 'v2funcs_prog 'v2funcs [])
+  in ltac2:(relcompile_tpe 'v2funcs_prog 'v2funcs ['v2func])
   as v2funcs_prog_proof.
 Proof.
   time relcompile.
 Qed.
 
 Derive vs2prog_prog
-  in ltac2:(relcompile_tpe 'vs2prog_prog 'vs2prog [])
+  in ltac2:(relcompile_tpe 'vs2prog_prog 'vs2prog ['v2funcs])
   as vs2prog_prog_proof.
 Proof.
   time relcompile.
@@ -162,16 +232,15 @@ Qed.
 (* entire parser *)
 
 Derive parser_prog
-  in ltac2:(relcompile_tpe 'parser_prog 'parser [])
+  in ltac2:(relcompile_tpe 'parser_prog 'parser ['parse; 'v2list; 'vs2prog])
   as parser_prog_proof.
 Proof.
   time relcompile.
 Qed.
 
 Derive str2imp_prog
-  in ltac2:(relcompile_tpe 'str2imp_prog 'str2imp [])
+  in ltac2:(relcompile_tpe 'str2imp_prog 'str2imp ['lexer; 'parser])
   as str2imp_prog_proof.
 Proof.
   time relcompile.
 Qed.
-
